

Proofs for Observable Propagation

Jacob Dunefsky

1 Proof of Theorem 1

Theorem 1. Define $f(x; n) = n \cdot \text{LayerNorm}(x)$. Define

$$\theta(x; n) = \arccos \left(\frac{n \cdot \nabla_x f(x; n)}{\|n\| \|\nabla_x f(x; n)\|} \right)$$

– that is, $\theta(x; n)$ is the angle between n and $\nabla_x f(x; n)$. Then if x and n are i.i.d. $\mathcal{N}(0, I)$ in \mathbb{R}^d , and $d \geq 8$ then

$$\mathbb{E} [\theta(x; n)] < 2 \arccos \left(\sqrt{1 - \frac{1}{d-1}} \right)$$

To prove this, we will introduce a lemma:

Lemma 1. Let y be an arbitrary vector. Let $A = I - \frac{vv^T}{\|v\|^2}$ be the orthogonal projection onto the hyperplane normal to v . Then the cosine similarity between y and Ay is given by $\sqrt{1 - \cos(\theta)^2}$, where $\cos(\theta)$ is the cosine similarity between y and v .

Proof. Assume without loss of generality that y is a unit vector. (Otherwise, we could rescale it without affecting the angle between y and v , or the angle between y and Ay .)

We have $Ay = y - \frac{y \cdot v}{\|v\|^2} v$. Then,

$$\begin{aligned} y \cdot Ay &= y \cdot \left(y - \frac{y \cdot v}{\|v\|^2} v \right) \\ &= \|y\|^2 - \frac{(y \cdot v)^2}{\|v\|^2} \\ &= 1 - \frac{(y \cdot v)^2}{\|v\|^2} \end{aligned}$$

and

$$\begin{aligned}
\|Ay\|^2 &= \left(y - \frac{y \cdot v}{\|v\|^2}v\right) \cdot \left(y - \frac{y \cdot v}{\|v\|^2}v\right) \\
&= y \cdot \left(y - \frac{y \cdot v}{\|v\|^2}v\right) - \frac{y \cdot v}{\|v\|^2}v \cdot \left(y - \frac{y \cdot v}{\|v\|^2}v\right) \\
&= y \cdot Ay - \frac{y \cdot v}{\|v\|^2}v \cdot \left(y - \frac{y \cdot v}{\|v\|^2}v\right) \\
&= y \cdot Ay - \frac{(y \cdot v)^2}{\|v\|^2} + \left\| \frac{y \cdot v}{\|v\|^2}v \right\|^2 \\
&= y \cdot Ay - \frac{(y \cdot v)^2}{\|v\|^2} + \frac{(y \cdot v)^2}{\|v\|^4} \|v\|^2 \\
&= y \cdot Ay - \frac{(y \cdot v)^2}{\|v\|^2} + \frac{(y \cdot v)^2}{\|v\|^2} \\
&= y \cdot Ay
\end{aligned}$$

Now, the cosine similarity between y and Ay is given by

$$\begin{aligned}
\frac{y \cdot Ay}{\|y\| \|Ay\|} &= \frac{y \cdot Ay}{\|Ay\|} \\
&= \frac{\|Ay\|^2}{\|Ay\|} \\
&= \|Ay\|
\end{aligned}$$

At this point, note that $\|Ay\| = \sqrt{y \cdot Ay} = \sqrt{1 - \frac{(y \cdot v)^2}{\|v\|^2}}$. But $\frac{y \cdot v}{\|v\|}$ is just the cosine similarity between y and v . Now, if we denote the angle between y and v by θ , we thus have

$$\|Ay\| = \sqrt{1 - \frac{(y \cdot v)^2}{\|v\|^2}} = \sqrt{1 - \cos(\theta)^2}.$$

□

Now, we are ready to prove Theorem 1.

Proof. First, observe that $\text{LayerNorm}(x) = \frac{Px}{\|Px\|}$, where $P = I - \frac{1}{d} \vec{1} \vec{1}^T$ is the orthogonal projection onto the hyperplane normal to $\vec{1}$, the vector of all ones. Thus, we have

$$f(x; n) = n^T \left(\frac{Px}{\|Px\|} \right)$$

Using the multivariate chain rule along with the rule that the derivative of $\frac{x}{\|x\|}$ is given by $\frac{I}{\|x\|} - \frac{xx^T}{\|x\|^3}$ (see section 2.6.1 of The Matrix Cookbook), we thus have that

$$\begin{aligned}
\nabla_x f(x; n) &= \left(n^T \left(\frac{I}{\|Px\|} - \frac{(Px)(Px)^T}{\|Px\|^3} \right) P \right)^T \\
&= \left(\frac{1}{\|Px\|} n^T \left(I - \frac{(Px)(Px)^T}{\|Px\|^2} \right) P \right)^T \\
&= \frac{1}{\|Px\|} P \left(I - \frac{(Px)(Px)^T}{\|Px\|^2} \right) n \quad \text{because } P \text{ is symmetric}
\end{aligned}$$

Denote $Q = I - \frac{(Px)(Px)^T}{\|Px\|^2}$. Note that this is an orthogonal projection onto the hyperplane normal to Px . We now have that $\nabla_x f(x; n) = \frac{1}{\|Px\|} PQn$. Because we only care about the angle between n and $\nabla_x f(x; n)$, it suffices to look at the angle between n and PQn , ignoring the $\frac{1}{\|Px\|}$ term.

Denote the angle between n and PQn as $\theta(x, n)$. (Note that θ is also a function of x because Q is a function of x .) Then if $\theta_Q(x, n)$ is the angle between n and Qn , and $\theta_P(x, n)$ is the angle between Qn and PQn , then $\theta(x, n) \leq \theta_Q(x, n) + \theta_P(x, n)$, so $\mathbb{E}[\theta(x, n)] \leq \mathbb{E}[\theta_Q(x, n)] + \mathbb{E}[\theta_P(x, n)]$.

Using Lemma 1, we have that $\theta_Q(x, n) = \arccos\left(\sqrt{1 - \cos(\phi(n, Px))^2}\right)$, where $\phi(n, Px)$ is the angle between n and Px . Now, because $n \sim \mathcal{N}(0, I)$, we have $\mathbb{E}[\cos(\phi(n, Px))^2] = 1/d$, using the well-known fact that the expected squared dot product between a uniformly distributed unit vector in \mathbb{R}^d and a given unit vector in \mathbb{R}^d is $1/d$.

At this point, define $g(t) = \arccos(\sqrt{1-t})$, $h(t) = g'\left(\frac{1}{d-1}\right)\left(t - \frac{1}{d-1}\right) + g\left(\frac{1}{d-1}\right)$. Then if $\frac{1}{d-1} < c$, where c is the least solution to $g'(c) = \frac{\pi - 2g(c)}{2(1-c)}$, then $h(t) \geq g(t)$. (Note that $g(t)$ is convex on $(0, 0.5]$ and concave on $[0.5, 1)$. Therefore, there are exactly two solutions to $g'(c) = \frac{\pi - 2g(c)}{2(1-c)}$. The lesser of the two solutions is the value at which $g'(c)$ equals the slope of the line between $(c, g(c))$ and $(1, \pi/2)$ – the latter point being the maximum of g – at the same time that $g''(c) \geq 0$.) One can compute $c \approx 0.155241\dots$, so if $d \geq 8$, then $1/(d-1) < c$ is satisfied, so $h(t) \geq g(t)$. Thus, we have the following inequality:

$$\begin{aligned}
h(1/(d-1)) &> h(1/d) \\
&= h(\mathbb{E}[\cos(\phi(n, Px))^2]) \\
&= \mathbb{E}[h(\cos(\phi(n, Px))^2)] \text{ due to linearity} \\
&\geq \mathbb{E}[g(\cos(\phi(n, Px))^2)] \text{ because } h(t) \geq g(t) \text{ for all } t \\
&= \mathbb{E}[\theta_Q(x, n)]
\end{aligned}$$

Now, $h(1/(d-1)) = g(1/(d-1)) = \arccos\left(\sqrt{1 - \frac{1}{d-1}}\right)$. Thus, we have that $\arccos\left(\sqrt{1 - \frac{1}{d-1}}\right) > \mathbb{E}[\theta_Q(x, n)]$.

The next step is to determine an upper bound for $\mathbb{E}[\theta_P(x, n)]$. By Lemma 1, we have that $\theta_P(x, n) = \arccos\left(\sqrt{1 - \cos(\phi(Qn, \vec{1}))^2}\right)$. Now, note that because $n \sim \mathcal{N}(0, I)$, then Qn is distributed according to a unit Gaussian in $\text{Im } Q$, the $(d-1)$ -dimensional hyperplane orthogonal to Px . Note that because $\vec{1}$ is orthogonal to Px (by the definition of P) and Px is orthogonal to $\text{Im } Q$, this means that $\vec{1} \in \text{Im } Q$. Now, let us apply the same fact from earlier: that the expected squared dot product between a uniformly distributed unit vector in \mathbb{R}^{d-1} and a given unit vector in \mathbb{R}^{d-1} is $1/(d-1)$. Thus, we have that $\mathbb{E}[\cos(\phi(Qn, \vec{1}))^2] = 1/(d-1)$.

From this, by the same logic as in the previous case, $\arccos\left(\sqrt{1 - \frac{1}{d-1}}\right) \geq \mathbb{E}[\theta_P(x, n)]$.

Adding this inequality to the inequality for $\mathbb{E}[\theta_Q(x, n)]$, we have

$$2 \arccos\left(\sqrt{1 - \frac{1}{d-1}}\right) > \mathbb{E}[\theta_Q(x, n)] + \mathbb{E}[\theta_P(x, n)] \geq \mathbb{E}[\theta(x, n)]$$

□

2 Proof of Theorem 2

Theorem 2. *Let $y_1, y_2 \in \mathbb{R}^d$. Let x be uniformly distributed on the hypersphere defined by the constraints $\|x\| = s$ and $x \cdot y_1 = k$. Then we have*

$$\mathbb{E}[x \cdot y_2] = k \frac{y_1 \cdot y_2}{\|y_1\|^2}$$

and the maximum and minimum values of $x \cdot y_2$ are given by

$$\frac{\|y_2\|}{\|y_1\|} \left(k \cos(\theta) \pm \sin(\theta) \sqrt{s^2 \|y_1\|^2 - k^2} \right)$$

where θ is the angle between y_1 and y_2 .

Before proving Theorem 2, we will prove a quick lemma.

Lemma 2. *Let \mathcal{S} be a hypersphere with radius r and center c . Then for a given vector y , the mean squared distance from y to the sphere, $\mathbb{E}_{s \in \mathcal{S}}[\|y - c\|^2]$, is given by $\|y - c\|^2 + r^2$.*

Proof. Without loss of generality, assume that \mathcal{S} is centered at the origin (so $\|y - c\|^2 = \|y\|^2$). Induct on the dimension of the \mathcal{S} . As our base case, let \mathcal{S} be the 0-sphere consisting of a point in \mathbb{R}^1 at $-r$ and a point at r . Then $\mathbb{E}_{s \in \mathcal{S}}[\|y - s\|^2] = \frac{(y-r)^2 + (y-(-r))^2}{2} = y^2 + r^2$.

For our inductive step, assume the inductive hypothesis for spheres of dimension $d-2$; we will prove the theorem of spheres of dimension $d-1$ in an ambient space of dimension d . Without loss of generality, let y lie on the x-axis,

so that we have $y = [y_1 \ 0 \ 0 \ \dots]^T$. Next, divide \mathcal{S} into slices along the x-axis. Denote the slice at position $x = x_0$ as \mathcal{S}_{x_0} . Then \mathcal{S}_{x_0} is a $(d-2)$ -sphere centered at $[x_0 \ 0 \ 0 \ \dots]^T$, and has radius $\sqrt{r^2 - x_0^2}$. Now, by the law of total expectation, $\mathbb{E}_{s \in \mathcal{S}}[\|y - s\|^2] = \mathbb{E}_{-r \leq x \leq r} [\mathbb{E}_{s' \in \mathcal{S}_x} [\|y - s'\|^2]]$. We then have that

$$\begin{aligned} \mathbb{E}_{s' \in \mathcal{S}_x} [\|y - s'\|^2] &= \mathbb{E} [(y_1 - x)^2 + s_2^2 + s_3^2 + \dots] \\ &= (y_1 - x)^2 + \mathbb{E} [s_2^2 + s_3^2 + \dots] \end{aligned}$$

Once again, \mathcal{S}_x is a $(d-2)$ -sphere defined by $s_2^2 + s_3^2 + \dots = r^2 - x^2$. This means that by the inductive hypothesis, we have $\mathbb{E} [s_2^2 + s_3^2 + \dots] = r^2 - x^2$. Thus, we have

$$\begin{aligned} \mathbb{E}_{s' \in \mathcal{S}_x} [\|y - s'\|^2] &= (y_1 - x)^2 + r^2 - x^2 \\ \mathbb{E}_{s' \in \mathcal{S}_x} [\|y - s'\|^2] &= (y_1 - x)^2 + r^2 - x^2 \\ \mathbb{E}_{s \in \mathcal{S}} [\|y - s\|^2] &= \mathbb{E}_{-r \leq x \leq r} [(y_1 - x)^2 + r^2 - x^2] \\ &= \frac{1}{2r} \int_{-r}^r (y_1 - x)^2 + r^2 - x^2 dx \\ &= r^2 + y_1^2 \end{aligned}$$

□

We are now ready to begin the main proof.

Proof. First, assume that $\|x\| = 1$. Now, the intersection of the $(d-1)$ -sphere defined by $\|x\| = 1$ and the hyperplane $x \cdot y_1 = k$ is a unit hypersphere of dimension $(d-2)$, oriented in the hyperplane $x \cdot y_1 = k$, and centered at $c_1 y_1$ where $c_1 = k / \|y_1\|^2$. Denote this $(d-2)$ -sphere as \mathcal{S} , and denote its radius by r .

Next, define $c_2 = \frac{k}{y_2 \cdot y_1}$. Then $c_2 y_2 \cdot y_1 = k$, so $c_2 y_2$ lies in the same hyperplane as \mathcal{S} . Additionally, because $c_1 y_1$ is in this hyperplane, and $c_1 y_1$ is also the normal vector for this hyperplane, we have that the vectors $c_1 y_1$, $c_2 y_2$, and $c_1 y_1 - c_2 y_2$ form a right triangle, where $c_2 y_2$ is the hypotenuse and $c_1 y_1 - c_2 y_2$ is the leg opposite of the angle θ between y_1 and y_2 . As such, we have that $\|c_1 y_1 - c_2 y_2\| = \sin(\theta) \|c_2 y_2\|$.

Furthermore, we have that $c_1 y_1 \cdot c_2 y_2 = \frac{k^2}{\|y_1\|^2}$, that $\|c_1 y_1\| = \frac{|k|}{\|y_1\|^2}$, and that $\|c_2 y_2\| = \frac{|k|}{\|y_1\| |\cos \theta|}$.

We will now begin to prove that the maximum and minimum values of $y_2 \cdot x$ are given by $\frac{\|y_2\|}{\|y_1\|} \left(k \cos(\theta) \pm |\sin(\theta)| \sqrt{s^2 \|y_1\|^2 - k^2} \right)$.

To start, note that the nearest point on \mathcal{S} to c_2y_2 and the farthest point on \mathcal{S} from c_2y_2 are located at the intersection of \mathcal{S} with the line between c_2y_2 and c_1y_1 .

To see this, let x_+ be the at the intersection of \mathcal{S} and the line between c_2y_2 and c_1y_1 . We will show that x_+ is the nearest point on \mathcal{S} to c_2y_2 . Let $x'_+ \in \mathcal{S} \neq x_+$. Then we have the following cases:

- Case 1: c_2y_2 is outside of \mathcal{S} . Then $\|c_2y_2 - c_1y_1\| = \|c_2y_2 - x_+\| + \|x_+ - c_1y_1\|$, because c_2y_2, x_+ , and c_1y_1 are collinear – so $\|c_2y_2 - c_1y_1\| = \|c_2y_2 - x_+\| + r$ (because $x_+ \in \mathcal{S}$). By the triangle inequality, we have $\|c_2y_2 - c_1y_1\| \leq \|c_2y_2 - x'_+\| + \|x'_+ - c_1y_1\| = \|c_2y_2 - x'_+\| + r$. But this means that $\|c_2y_2 - x_+\| \leq \|c_2y_2 - x'_+\|$.
- Case 2: c_2y_2 is inside of \mathcal{S} . Then $\|c_2y_2 - c_1y_1\| = \|x_+ - c_1y_1\| - \|c_2y_2 - x_+\|$, because c_2y_2, x_+ , and c_1y_1 are collinear – so $\|c_2y_2 - c_1y_1\| = r - \|c_2y_2 - x_+\|$. By the triangle inequality, we have $\|x'_+ - c_1y_1\| \leq \|c_2y_2 - x'_+\| + \|c_2y_2 - c_1y_1\|$, so $\|x'_+ - c_1y_1\| \leq \|c_2y_2 - x'_+\| + r - \|c_2y_2 - x_+\|$. But since $\|x'_+ - c_1y_1\| = r$, this means that $\|c_2y_2 - x_+\| \leq \|c_2y_2 - x'_+\|$.

A similar argument will show that x_- , the farthest point on \mathcal{S} from c_2y_2 , is also located at the intersection of \mathcal{S} with the line between c_2y_2 and c_1y_1 .

Now, let us find the values of x_+ and x_- . The line between c_2y_2 and c_1y_1 can be parameterized by a scalar t as $c_1y_1 + t(c_2y_2 - c_1y_1)$. Then x_+ and x_- are given by $c_1y_1 + t^*(c_2y_2 - c_1y_1)$, where t^* are the solutions to the equation $\|c_1y_1 + t(c_2y_2 - c_1y_1)\| = 1$.

We have the following:

$$\begin{aligned}
1 &= \|c_1y_1 + t(c_2y_2 - c_1y_1)\| \\
&= \|c_1y_1\|^2 + 2t(c_1y_1 \cdot (c_2y_2 - c_1y_1)) + t^2 \|c_2y_2 - c_1y_1\|^2 \\
&= \|c_1y_1\|^2 + 2t((c_1y_1 \cdot c_2y_2) - \|c_1y_1\|^2) + t^2 \|c_2y_2\|^2 \sin^2 \theta \\
&= \frac{k^2}{\|y_1\|^2} + 2t \left(\frac{k^2}{\|y_1\|^2} - \frac{k^2}{\|y_1\|^2} \right) + t^2 \frac{k^2}{\|y_1\|^2 \cos^2 \theta} \sin^2 \theta \\
&= \frac{k^2}{\|y_1\|^2} (t^2 \tan^2 \theta + 1)
\end{aligned}$$

Thus, solving for t , we have that $t^* = \frac{\pm \sqrt{\|y_1\|^2 - k^2}}{|k| \tan \theta}$. Therefore, we have that

$$\begin{aligned}
x_+, x_- &= c_1 y_1 + t^*(c_2 y_2 - c_1 y_1) \\
&= c_1 y_1 + \left(\frac{k^2}{\|y_1\|^2} (t^2 \tan^2 \theta + 1) \right) (c_2 y_2 - c_1 y_1) \\
&= \frac{k y_1}{\|y_1\|^2} + \left(\frac{\pm \sqrt{\|y_1\|^2 - k^2}}{|k| \tan \theta} \right) \left(\frac{k y_2}{y_1 \cdot y_2} - \frac{k y_1}{\|y_1\|^2} \right) \\
&= k \left[\frac{y_1}{\|y_1\|^2} \pm \left(\frac{\sqrt{\|y_1\|^2 - k^2}}{|k| \tan \theta} \right) \left(\frac{y_2}{y_1 \cdot y_2} - \frac{y_1}{\|y_1\|^2} \right) \right] \\
y_2 \cdot x_+, y_2 \cdot x_- &= y_2 \cdot k \left[\frac{y_1}{\|y_1\|^2} \pm \left(\frac{\sqrt{\|y_1\|^2 - k^2}}{|k| \tan \theta} \right) \left(\frac{y_2}{y_1 \cdot y_2} - \frac{y_1}{\|y_1\|^2} \right) \right] \\
&= \frac{k y_1 \cdot y_2}{\|y_1\|^2} \pm \left(\cot \theta \sqrt{\|y_1\|^2 - k^2} \right) \left(\frac{y_2 \cdot y_2}{y_1 \cdot y_2} - \frac{y_1 \cdot y_1}{\|y_1\|^2} \right) \\
&= \frac{k y_1 \cdot y_2}{\|y_1\|^2} \pm \left(\cot \theta \sqrt{\|y_1\|^2 - k^2} \right) \left(\frac{\|y_2\|}{\|y_1\| \cos \theta} - \frac{\|y_2\| \cos \theta}{\|y_1\|} \right) \\
&= \left[\frac{k y_1 \cdot y_2}{\|y_1\|^2} \pm \left(\cot \theta \sqrt{\|y_1\|^2 - k^2} \right) \frac{\|y_2\|}{\|y_1\|} \left(\frac{1}{\cos \theta} - \cos \theta \right) \right] \\
&= \frac{k y_1 \cdot y_2}{\|y_1\|^2} \pm \left(\cot \theta \sqrt{\|y_1\|^2 - k^2} \right) \frac{\|y_2\|}{\|y_1\|} \sin \theta \tan \theta \\
&= \frac{k y_1 \cdot y_2}{\|y_1\|^2} \pm \frac{\|y_2\|}{\|y_1\|} \sin \theta \sqrt{\|y_1\|^2 - k^2} \\
&= \frac{\|y_2\|}{\|y_1\|} \left(k \cos(\theta) \pm \sin(\theta) \sqrt{\|y_1\|^2 - k^2} \right)
\end{aligned}$$

We will now prove that $\mathbb{E}[y_2 \cdot x] = \frac{y_1 \cdot y_2}{\|y_1\|^2}$. Before we do, note that we can also use our value of t^* to determine the squared radius of \mathcal{S} . We have that the squared radius of \mathcal{S} is given by

$$\begin{aligned}
r^2 &= \|t^*(c_2 y_2 - c_1 y_1)\|^2 \\
&= (t^*)^2 \|(c_2 y_2 - c_1 y_1)\|^2 \\
&= (t^*)^2 \sin^2 \theta \|c_2 y_2\|^2 \\
&= \frac{\sin^2(\theta) k^2 / (\|y_1\|^2 \cos^2 \theta)}{k^2 \tan \theta} (\|y_1\|^2 - k^2) \\
&= 1 - \frac{k^2}{\|y_1\|^2}
\end{aligned}$$

We will use this result soon. Now, on to the main event. Begin by noting that $y_2 \cdot x = \|y_2\| \|x\| \cos(y_2, x) = \|y_2\| \cos(y_2, x)$, where $\cos(y_2, x)$ is the cosine of the angle between y_2 and x . Now, $\cos(y_2, x) = \text{signum}(c_2) \cos(c_2 y_2, x)$. And we have that $\|x - c_2 y_2\|^2 = \|x\|^2 + \|c_2 y_2\|^2 - 2 \|x\| \|c_2 y_2\| \cos(c_2 y_2, x) = 1 + \|c_2 y_2\|^2 - 2 \|c_2 y_2\| \cos(c_2 y_2, x)$. Therefore, we have

$$\begin{aligned} \cos(y_2, x) &= \text{signum}(c_2) \cos(c_2 y_2, x) \\ &= \text{signum}(c_2) \frac{\|x - c_2 y_2\|^2 - 1 - \|c_2 y_2\|^2}{-2 \|c_2 y_2\|} \\ &= \text{signum}(c_2) \frac{1 + \|c_2 y_2\|^2 - \|x - c_2 y_2\|^2}{2 \|c_2 y_2\|} \end{aligned}$$

$$\begin{aligned} y_2 \cdot x &= \|y_2\| \cos(y_2, x) \\ &= \text{signum}(c_2) \|y_2\| \frac{1 + \|c_2 y_2\|^2 - \|x - c_2 y_2\|^2}{2 \|c_2 y_2\|} \end{aligned}$$

$$\begin{aligned} \mathbb{E}[y_2 \cdot x] &= \mathbb{E} \left[\text{signum}(c_2) \|y_2\| \frac{1 + \|c_2 y_2\|^2 - \|x - c_2 y_2\|^2}{2 \|c_2 y_2\|} \right] \\ &= \text{signum}(c_2) \|y_2\| \frac{1 + \|c_2 y_2\|^2 - \mathbb{E}[\|x - c_2 y_2\|^2]}{2 \|c_2 y_2\|} \\ &= \text{signum}(c_2) \|y_2\| \frac{1 + \|c_2 y_2\|^2 - \left(1 - \frac{k^2}{\|y_1\|^2} + \|c_1 y_1 - c_2 y_2\|^2\right)}{2 \|c_2 y_2\|} \end{aligned}$$

This last line uses Lemma 2: $c_1 y_1$ is the center of \mathcal{S} , so the expected squared distance between $c_2 y_2$ and a point on \mathcal{S} is given by $1 - \frac{k^2}{\|y_1\|^2} + \|c_1 y_1 - c_2 y_2\|^2$, where $1 - \frac{k^2}{\|y_1\|^2}$ is the squared radius of \mathcal{S} and $\|c_1 y_1 - c_2 y_2\|^2$ is the squared distance from $c_2 y_2$ to the center. We can use this lemma because $c_2 y_2$ is in the same hyperplane as \mathcal{S} , so we can treat this situation as being set in a space of dimension $d - 1$.

Now, continue to simplify:

$$\begin{aligned}
\mathbb{E}[y_2 \cdot x] &= \text{signum}(c_2) \|y_2\| \frac{1 + \|c_2 y_2\|^2 - \left(1 - \frac{k^2}{\|y_1\|^2} + \|c_1 y_1 - c_2 y_2\|^2\right)}{2 \|c_2 y_2\|} \\
&= \text{signum}(c_2) \|y_2\| \frac{\|c_2 y_2\|^2 + \frac{k^2}{\|y_1\|^2} - \sin^2 \theta \|c_2 y_2\|^2}{2 \|c_2 y_2\|} \\
&= \text{signum}(c_2) \|y_2\| \frac{\|c_2 y_2\|^2 \cos^2 \theta + \frac{k^2}{\|y_1\|^2}}{2 \|c_2 y_2\|} \\
&= \text{signum}(c_2) \|y_2\| \frac{1}{2} \left(\|c_2 y_2\| \cos^2 \theta + \frac{|k| \cos \theta}{\|y_1\|} \right) \\
&= \text{signum}(c_2) \|y_2\| \frac{1}{2} \left(\frac{|k| |\cos \theta|}{\|y_1\|} + \frac{|k| |\cos \theta|}{\|y_1\|} \right) \\
&= \text{signum}(c_2) |k| \frac{\|y_2\|}{\|y_1\|} |\cos \theta| \\
&= k \frac{\|y_2\|}{\|y_1\|} \cos \theta \\
&= k \frac{y_1 \cdot y_2}{\|y_1\|^2}
\end{aligned}$$

The last thing to do is to note that the above formulas are only valid when $\|x\| = 1$. But if $\|x\| = s$, this is equivalent to the case when $\|x\| = 1$ if we scale y_1 and y_2 by s . Scaling those two vectors by s gives us the final formulas in Theorem 2. \square